src/ldrfra/PFtoRASimThread.v
@@ -25,6 +25,7 @@ Require Import MemoryMerge.
 
 Require Import PFStep.
 Require Import OrdStep.
+Require Import Writes.
 Require Import WStep.
 Require Import Stable.
 
@@ -36,49 +37,6 @@ Module PFtoRASimThread.
     Variable lang: language.
     Variable L: Loc.t -> bool.
 
-    (* stable *)
-
-    Inductive normal_thread (e: Thread.t lang): Prop :=
-    | normal_thread_intro
-        (NORMAL_TVIEW: Stable.normal_tview L (Local.tview (Thread.local e)))
-        (NORMAL_MEMORY: Stable.normal_memory L (Thread.memory e))
-    .
-    Hint Constructors normal_thread.
-
-    Inductive stable_thread (rels: RelWrites.t) (e: Thread.t lang): Prop :=
-    | stable_thread_intro
-        (STABLE_TVIEW: Stable.stable_tview L (Thread.memory e) (Local.tview (Thread.local e)))
-        (STABLE_SC: Stable.stable_timemap L (Thread.memory e) (Thread.sc e))
-        (STABLE_MEMORY: Stable.stable_memory L rels (Thread.memory e))
-    .
-    Hint Constructors stable_thread.
-
-    Lemma future_normal_thread
-          e sc' mem'
-          (NORMAL: normal_thread e)
-          (NORMAL_MEM: Stable.normal_memory L mem'):
-      normal_thread (Thread.mk lang (Thread.state e) (Thread.local e) sc' mem').
-    Proof.
-      inv NORMAL. econs; ss.
-    Qed.
-
-    Lemma future_stable_thread
-          rels e sc' mem'
-          (WF: Local.wf (Thread.local e) (Thread.memory e))
-          (STABLE: stable_thread rels e)
-          (SC: TimeMap.le (Thread.sc e) sc')
-          (MEM: Memory.future (Thread.memory e) mem')
-          (STABLE_SC: Stable.stable_timemap L mem' sc')
-          (STABLE_MEM: Stable.stable_memory L rels mem'):
-      stable_thread rels (Thread.mk lang (Thread.state e) (Thread.local e) sc' mem').
-    Proof.
-      destruct e, local. inv STABLE. inv WF. ss.
-      econs; i; ss; eauto using Stable.future_stable_tview.
-    Qed.
-
-
-    (* sim *)
-
     Inductive sim_tview (tview_src tview_tgt: TView.t): Prop :=
     | sim_tview_intro
         (REL: forall loc, if L loc
@@ -88,13 +46,11 @@ Module PFtoRASimThread.
         (ACQ: (TView.acq tview_src) = (TView.acq tview_tgt))
     .
 
-    Inductive sim_local (rels: RelWrites.t) (lc_src lc_tgt: Local.t): Prop :=
+    Inductive sim_local (rels: Writes.t) (lc_src lc_tgt: Local.t): Prop :=
     | sim_local_intro
         (TVIEW: sim_tview (Local.tview lc_src) (Local.tview lc_tgt))
         (PROMISES: (Local.promises lc_src) = (Local.promises lc_tgt))
         (RESERVE: OrdLocal.reserve_only L (Local.promises lc_src))
-        (REL_WRITES_NONE: forall loc to (IN: List.In (loc, to) rels),
-            Memory.get loc to (Local.promises lc_src) = None)
     .
 
     Inductive sim_message (loc: Loc.t): forall (msg_src msg_tgt: Message.t), Prop :=
@@ -104,6 +60,8 @@ Module PFtoRASimThread.
         sim_message loc (Message.concrete val released_src) (Message.concrete val released_tgt)
     | sim_message_reserve:
         sim_message loc Message.reserve Message.reserve
+    | sim_message_undef:
+        sim_message loc Message.undef Message.undef
     .
 
     Program Instance sim_message_PreOrder: forall loc, PreOrder (sim_message loc).
@@ -114,7 +72,7 @@ Module PFtoRASimThread.
       ii. inv H; inv H0; ss; econs; eauto. des_ifs. etrans; eauto.
     Qed.
 
-    Inductive sim_memory (rels: RelWrites.t) (mem_src mem_tgt: Memory.t): Prop :=
+    Inductive sim_memory (rels: Writes.t) (mem_src mem_tgt: Memory.t): Prop :=
     | sim_memory_intro
         (SOUND: forall loc from to msg_src
                   (GET_SRC: Memory.get loc to mem_src = Some (from, msg_src)),
@@ -126,13 +84,13 @@ Module PFtoRASimThread.
             exists msg_src,
               <<GET_SRC: Memory.get loc to mem_src = Some (from, msg_src)>> /\
               <<MSG: sim_message loc msg_src msg_tgt>>)
-        (REL_WRITES: forall loc to (IN: List.In (loc, to) rels),
+        (REL_WRITES: forall loc to ord (IN: List.In (loc, to, ord) rels),
             exists from val released,
               <<GET_SRC: Memory.get loc to mem_src = Some (from, Message.concrete val (Some released))>> /\
               <<GET_TGT: Memory.get loc to mem_tgt = Some (from, Message.concrete val (Some released))>>)
     .
 
-    Inductive sim_statelocal (rels: RelWrites.t):
+    Inductive sim_statelocal (rels: Writes.t):
       forall (sl_src sl_tgt: {lang : language & Language.state lang} * Local.t), Prop :=
     | sim_statelocal_intro
         lang st lc_src lc_tgt
@@ -141,7 +99,7 @@ Module PFtoRASimThread.
     .
     Hint Constructors sim_statelocal.
 
-    Inductive sim_thread (rels: RelWrites.t) (e_src e_tgt: Thread.t lang): Prop :=
+    Inductive sim_thread (rels: Writes.t) (e_src e_tgt: Thread.t lang): Prop :=
     | sim_thread_intro
         (STATE: (Thread.state e_src) = (Thread.state e_tgt))
         (LOCAL: sim_local rels (Thread.local e_src) (Thread.local e_tgt))
@@ -480,8 +438,8 @@ Module PFtoRASimThread.
           rels lc_src lc_tgt mem_src mem_tgt
           (LC: sim_local rels lc_src lc_tgt)
           (MEM: sim_memory rels mem_src mem_tgt):
-      <<RELS_WF_SRC: RelWrites.wf rels (Local.promises lc_src) mem_src>> /\
-      <<RELS_WF_TGT: RelWrites.wf rels (Local.promises lc_tgt) mem_tgt>>.
+      <<RELS_WF_SRC: Writes.wf rels (Local.promises lc_src) mem_src>> /\
+      <<RELS_WF_TGT: Writes.wf rels (Local.promises lc_tgt) mem_tgt>>.
     Proof.
       inv LC. inv MEM. split; ii.
       - exploit REL_WRITES; eauto. i. des. esplits; eauto.
@@ -1572,9 +1530,9 @@ Module PFtoRASimThread.
       exists e_src e2_src,
         (<<STEP_SRC: OrdThread.step L Ordering.acqrel pf e_src e1_src e2_src>>) /\
         __guard__ (
-            (<<SIM2: sim_thread (RelWrites.append L e_src rels) e2_src e2_tgt>>) /\
+            (<<SIM2: sim_thread (Writes.append L e_src rels) e2_src e2_tgt>>) /\
             (<<EVENT: sim_event e_src e_tgt>>) /\
-            (<<STABLE2_SRC: stable_thread (RelWrites.append L e_src rels) e2_src>>) /\
+            (<<STABLE2_SRC: stable_thread (Writes.append L e_src rels) e2_src>>) /\
             (<<NORMAL2_SRC: normal_thread e2_src>>) /\
             (<<NORMAL2_TGT: normal_thread e2_tgt>>)
             \/
@@ -1623,7 +1581,7 @@ Module PFtoRASimThread.
         + hexploit write_step_loc; try exact LOCAL0; eauto; ss. i. des.
           esplits.
           * econs 2. econs; [|econs 3]; eauto.
-          * left. rewrite REL in *. unfold RelWrites.append. ss. rewrite LOC.
+          * left. rewrite REL in *. unfold Writes.append. ss. rewrite LOC.
             esplits; ss. econs; ss. inv STEP_SRC.
             exploit Local.write_step_future; try eapply STEP; eauto. i. des.
             inv STEP. ss.
@@ -1632,7 +1590,7 @@ Module PFtoRASimThread.
           { apply Stable.bot_stable_view. ss. }
           i. des. esplits.
           * econs 2. econs; [|econs 3]; eauto.
-          * left. unfold RelWrites.append. ss. rewrite LOC.
+          * left. unfold Writes.append. ss. rewrite LOC.
             esplits; ss. econs; ss. inv STEP_SRC.
             exploit Local.write_step_future; try eapply STEP; eauto. i. des.
             inv STEP. ss.
@@ -1655,7 +1613,7 @@ Module PFtoRASimThread.
             i. des. esplits.
             { econs 2. econs; [|econs 4]; eauto. }
             { left. rewrite REL in *.
-              unfold RelWrites.append. ss. rewrite LOC in *.
+              unfold Writes.append. ss. rewrite LOC in *.
               esplits; ss. econs; ss.
               inv STEP_SRC0. exploit Local.write_step_future; try exact STEP; eauto. i. des.
               inv STEP. ss.
@@ -1816,7 +1774,7 @@ Module PFtoRASimThread.
             eapply STABLE_MEMORY; eauto. left. congr. }
           i. des. esplits.
           * econs 2. econs; [|econs 4]; eauto.
-          * left. unfold RelWrites.append. ss. rewrite LOC.
+          * left. unfold Writes.append. ss. rewrite LOC.
             esplits; ss. econs; ss.
             inv STEP_SRC0.
             exploit Local.write_step_future; try exact STEP0; eauto. i. des.
